\input{../../doc}
\input{../../preamb}
\input{../eng}

\begin{document}	
\vedlegg{Solving equations by variable substitution} \label{Bytvar}
Let us solve the equation 
\begin{equation}\label{eqsqrtxu}
	x-11\sqrt{x}+28=0
\end{equation}
Upon closer inspection, we realize that this is a quadratic equation for $ \sqrt{x} $. This becomes even clearer if we define the variable $ u=\sqrt{x} $, then we can write \eqref{eqsqrtxu} as
\[ u^2-11u+28=0 \]
Since $ (-7)\cdot(-4)=28 $ and $ -7-4=-11 $, we have from \eqref{a1a2eq} that
\[ (u-4)(u-7)=0 \]
Thus,
\[ u=4 \qquad \vee \qquad u=7 \]
This means that
\[ \sqrt{x}=4 \qquad \vee \qquad \sqrt{x}=7 \]
Therefore,
\[ x=16 \qquad \vee \qquad x=49 \]


\end{document}